Locale.thy
@@ -11,6 +11,7 @@ fixes delete :: "'a \<Rightarrow> 't \<Rightarrow> 't"
 fixes lookup :: "'t \<Rightarrow> 'a \<Rightarrow> bool"
 fixes  invar :: "'t \<Rightarrow> bool"
 fixes  to_set:: "'t \<Rightarrow> 'a set"
+fixes  is_sub:: "'a \<Rightarrow> 'a \<Rightarrow> bool"
 fixes  match :: "'t \<Rightarrow> 'a \<Rightarrow> 'a list"
 
 assumes  invar_empty:  "invar empty"
@@ -18,12 +19,13 @@ assumes invar_insert: "invar t \<Longrightarrow> invar(insert x t)"
 assumes invar_delete: "invar t \<Longrightarrow> invar(delete x t)"
 assumes   insert_set:   "to_set (insert x t) = to_set t \<union> {x}"
 assumes   delete_set:   "invar t \<Longrightarrow> to_set (delete x t) = to_set t - {x}"
-assumes match_correctness: " \<forall>xl\<in>set (match t l). lookup t xl"
+assumes match_correctness: " \<forall>xl\<in>set (match t l). (lookup t xl) \<and> is_sub xl l"
 
 
 interpretation FMPM: Match
-where empty = empty_trie and lookup = lookup_trie and insert = insert_trie and delete = delete_trie
-and invar = invar_trie and to_set = trie_set and match = FMPM
+  where empty = empty_trie and lookup = lookup_trie and insert = insert_trie 
+  and delete = delete_trie and invar = invar_trie and to_set = trie_set 
+  and is_sub = is_Substring and match = FMPM
 proof (standard, goal_cases)
   case 1
   then show ?case by (simp add:empty_trie_def)
